small extra syntax + Branch pattern + rework of Head and BlockFusion

theories/Block.v
@@ -7,13 +7,12 @@ From Pattern Require Import IdModule MapCFG.
 Import Map MapF MapF.P MapF.P.F.
 Import IdOT MapCFG.
 
-
 Definition blocks_aux (G: map_cfg) : _ -> (blk*map_cfg) := fun '(id, b) => (b, remove id G).
 
 Definition blocks (G: map_cfg): list (blk*map_cfg) := List.map (blocks_aux G) (elements G).
 
-Definition is_block (G G': map_cfg) b := MapsTo b.(blk_id) b G /\ G' ≡ (remove b.(blk_id) G).
+Definition block_sem (G G': map_cfg) b := MapsTo_id b G /\ G' ≡ (remove_id b G) /\ wf_map_cfg G'.
 
-Lemma blocks_correct: forall G G' b, wf_map_cfg G -> ((b, G') ∈ (blocks G) <-> is_block G G' b).
+Lemma blocks_correct: forall G G' b, wf_map_cfg G -> ((b, G') ∈ (blocks G) <-> block_sem G G' b).
 Proof.
 Admitted.
