theories/BlockFusion.v
@@ -1,22 +1,21 @@
+(* Block Fusion using the Block pattern *)
+
 From Vellvm Require Import Syntax ScopeTheory Semantics.
 From ITree Require Import ITree Eq.
-From Pattern Require Import IdModule MapCFG Head Focus Patterns.
+From Pattern Require Import IdModule MapCFG Patterns.
 Require Import FSets.FMapAVL FSets.FMapFacts.
 Require Import List.
 Import ListNotations.
 Import Map MapF MapF.P MapF.P.F.
-Import IdOT MapCFG Head Focus Patterns.
+Import IdOT MapCFG Head Focus Block Patterns.
 
 Definition is_seq (A B: blk) := match successors A with
   | [x] => eqb x B.(blk_id)
   | _ => false
 end.
 
-Definition DoubleHead {S} (P: Pat S) := 
-  (Head (Head P)) when (fun '(A,(B,_)) => is_seq A B).
-
 Definition BlockFusion {S} (P: Pat S) :=
-  (Focus (DoubleHead P)) when (fun '(G,(_,(B,_))) => is_empty (predecessors B.(blk_id) G)).
+    (Block (Head P)) when (fun '(A, (B, _)) => is_seq A B).
 
 Lemma is_seq_correct:
   forall A B, is_seq A B = true <->
@@ -28,105 +27,36 @@ Proof.
   rewrite H. now apply eqb_eq.
 Qed.
 
-Definition DoubleHead_sem A B G G' := let G'' := (add B.(blk_id) B G') in
-  successors A = [B.(blk_id)] /\
-  (predecessors B.(blk_id) G) ≡ (add A.(blk_id) A empty) /\
-  G ≡ (add A.(blk_id) A G'') /\
-  is_head G G'' A /\ is_head G'' G' B.
+Definition BlockFusion_sem A B G G' :=
+  G' ≡ (remove_id B (remove_id A G)) /\ ~(A.(blk_id) === B.(blk_id)) /\
+  MapsTo_id A G /\ MapsTo_id B G /\
+  (predecessors B.(blk_id) G) ≡ (single A) /\ successors A = [B.(blk_id)].
 
-Theorem Pat_DoubleHead_correct {S}: forall A B G (P:Pat S) X,
-  wf_map_cfg G -> (A,(B,X)) ∈ (MatchAll (DoubleHead P) G) <->
-  exists G', X ∈ (MatchAll P G') /\ DoubleHead_sem A B G G'.
+Theorem Pat_BlockFusion_correct {S}: forall A B G (P: Pat S) X, wf_map_cfg G ->
+  (A, (B, X)) ∈ (MatchAll (BlockFusion P) G) <->
+  exists G1, X ∈ (MatchAll P G1) /\ BlockFusion_sem A B G G1.
 Proof.
-  intros A B G P X Hwf. unfold DoubleHead. split.
-  - intro H.
-    apply Pat_When_correct in H as [H HWhen].
-    apply Pat_Head_correct in H as [G1 [[HRA [HwfA [HMA HPA]]] H]]; trivial.
-    apply Pat_Head_correct in H as [G2 [[HRB [HwfB [HMB HPB]]] H]]; trivial.
-    apply is_seq_correct in HWhen.
+  intros A B G P X Hwf. unfold BlockFusion. split.
+  - intros H.
+    apply Pat_When_correct in H as [H Hseq]. apply is_seq_correct in Hseq.
+    apply Pat_Block_correct in H as [G1 [[HmA [HrA Hwf1]] H]]; trivial.
+    apply Pat_Head_correct in H as [G2 [[HrB [Hwf2 [HmB Hp]]] H]]; trivial.
     exists G2. split; trivial.
     repeat split; trivial.
-    * apply add_predecessor; trivial. eapply Empty_m. unfold predecessors.
-      eapply fold_Equal; auto.
-      + symmetry. apply HRA.
-      + trivial.
-    * apply add_remove_elim2. trivial.
-      etransitivity. 2:apply HRA.
-      symmetry. now apply add_remove_elim2.
-    * etransitivity. 2:apply HRA. symmetry. now apply add_remove_elim2.
-    * eapply wf_map_cfg_eq. 2:apply HwfA. now apply add_remove_elim2.
-    * etransitivity. apply HRB. apply remove_m. reflexivity. now apply add_remove_elim2.
-    * apply add_1. reflexivity.
-    * eapply Empty_m. 2: apply HPB. unfold predecessors. apply fold_Equal; auto.
-      symmetry. now apply add_remove_elim2.
-  - intros [G' [HG' [Hs [Hp [He [HhA HhB]]]]]].
-    apply Pat_When_correct. split. apply Pat_Head_correct; trivial.
-    exists (add (blk_id B) B G'). split. trivial.
-    apply Pat_Head_correct. apply add_wf_map_cfg. destruct HhB as [HB1 [HB2 [HB3 HB4]]]. trivial.
-    exists G'. split; trivial.
-    unfold is_seq. rewrite Hs. now apply eqb_eq.
+    * etransitivity. apply HrB. now apply remove_m.
+    * eapply remove_mapsto_iff. eapply MapsTo_m. reflexivity. reflexivity. symmetry.
+      apply HrA. apply HmB.
+    * eapply remove_3. eapply MapsTo_m. reflexivity. reflexivity. symmetry. apply HrA. trivial.
+    * eapply add_predecessor; trivial. etransitivity.
+      2: {apply Eempty. apply Hp. }
+      apply filter_m; auto. now symmetry.
+  - intros [G2 [HX [H2 [HmA [HmB [Hne [Hp Hs]]]]]]]. remember (remove_id A G) as G1.
+    apply Pat_When_correct. rewrite is_seq_correct. split; trivial.
+    apply Pat_Block_correct; trivial. exists G1. subst.
+    repeat split; trivial. now apply remove_wf_map_cfg.
+    apply Pat_Head_correct. now apply remove_wf_map_cfg.
+    exists G2. repeat split; trivial.
+    * eapply wf_map_cfg_eq. symmetry. apply H2. now repeat apply remove_wf_map_cfg.
+    * now eapply remove_2.
+    * apply Eempty. etransitivity. apply remove_predecessor; trivial. reflexivity.
 Qed.
-
-Definition BlockFusion_sem A B G G' G'' := let G2 := (add A.(blk_id) A (add B.(blk_id) B G')) in
-  (predecessors B.(blk_id) G) ≡ (add A.(blk_id) A empty) /\
-  Partition G G'' G2 /\ DoubleHead_sem A B G2 G'.
-
-Theorem Pat_BlockFusion_correct {S}: forall A B G G'' (P: Pat S) X, wf_map_cfg G ->
-  (G'', (A, (B, X))) ∈ (MatchAll (BlockFusion P) G) <->
-  exists G', X ∈ (MatchAll P G') /\ BlockFusion_sem A B G G' G''.
-Proof.
-  unfold BlockFusion.
-  intros A B G G'' P X Hwf. split.
-  - intro H. unfold BlockFusion_sem.
-    apply Pat_When_correct in H as [H HWhen].
-    apply Pat_Focus_correct in H as [G0 [[HPart [Hwf'' Hwf0]] H]]; trivial.
-    apply Pat_DoubleHead_correct in H as [G' [ HG' [HS [HP [HG0 [HhA HhB]]]]]]; trivial.
-    exists G'. split; trivial.
-    remember (add (blk_id A) A (add (blk_id B) B G')) as G2. 
-    split. 2:split. 3:split; trivial. 3:split. 4:split. 5:split;trivial.
-    * unfold predecessors. etransitivity.
-    2:apply HP. etransitivity. 2: {
-      unfold predecessors. eapply fold_Equal2; auto. reflexivity.
-      apply Eempty. apply is_empty_iff. apply HWhen.
-    }
-    unfold predecessors. apply Partition_fold; auto. now apply Partition_sym.
-    * eapply Partition_m. reflexivity. reflexivity. symmetry. apply HG0. trivial.
-    * etransitivity. 2:apply HP. unfold predecessors. symmetry. apply fold_Equal;auto.
-    * rewrite HeqG2. reflexivity.
-    * eapply is_head_eq. apply HG0. reflexivity. trivial.
-  - intros [G' [HG' [Hpred [Hpart HDouble]]]].
-    remember (add (blk_id A) A (add (blk_id B) B G')) as G2.
-    apply Pat_When_correct. split.
-    apply Pat_Focus_correct; trivial.
-    exists G2. split.
-    destruct HDouble as [HSucc [HPred2 [_ [HhA HhB]]]].
-    split; trivial. eapply wf_map_cfg_part. apply Hpart. trivial.
-    apply Pat_DoubleHead_correct. eapply wf_map_cfg_part. apply Hpart. trivial.
-    exists G'. split; trivial.
-    apply is_empty_1. intros k e H.
-    induction (eq_dec k A.(blk_id)) as [a|a].
-    * apply eq_eq in a. subst k.
-      destruct Hpart as [HD HM].
-      eapply HD. split. 2:{ rewrite HeqG2. apply add_in_iff. left. reflexivity. }
-      eapply predecessors_in. apply in_mapsto_iff. exists e. apply H.
-    * destruct HDouble as [Hsucc [Hpred2 HDouble]].
-      assert (Hn: In k (predecessors (blk_id B) G)).
-      eapply In_m. reflexivity.
-      assert (Heq: (predecessors (blk_id B) G) ≡
-                   (fold (predecessors_aux (B.(blk_id))) G''
-                         (fold (predecessors_aux (B.(blk_id))) G2 empty))
-             ).
-      unfold predecessors.
-      apply Partition_fold; auto.
-      apply Heq. apply predecessors_aux_empty_acc. apply in_mapsto_iff. now exists e.
-      eapply empty_in_iff.
-      eapply add_neq_in_iff. apply neq_sym. apply a.
-      eapply In_m. reflexivity. symmetry. apply Hpred. trivial. 
-Qed.
-
-(* Theorem FusionCorrect (G G' G'':map_cfg) A B f to:
-  wf_map_cfg G -> to <> B.(blk_id) -> f <> A.(blk_id) ->
-  (G'', (A, (B, G'))) ∈ (MatchAll (BlockFusion □) G) ->
-  denotation_map_cfg G (f, to) ≈
-  denotation_map_cfg (update (update G G') (single (fusion A B))) (f, to).
-Admitted. *)
