theories/Head.v
@@ -9,13 +9,10 @@ Import IdOT MapCFG.
 
 (* Head Definitions *)
 
-Definition predecessors_aux (b id: bid) (bk: blk) acc :=
-  if is_predecessor b bk
-  then add id bk acc
-  else acc.
+Definition predecessors_aux (b id: bid) (bk: blk) := is_predecessor b bk.
 
 Definition predecessors (b : bid) (G : map_cfg) : map_cfg :=
-    fold (predecessors_aux b) G empty.
+    filter (predecessors_aux b) G.
 
 Definition heads_aux (G: map_cfg) id b acc : list (blk*map_cfg) :=
   if is_empty (predecessors id G)
@@ -24,108 +21,60 @@ Definition heads_aux (G: map_cfg) id b acc : list (blk*map_cfg) :=
 
 Definition heads (G: map_cfg): list (blk*map_cfg) := fold (heads_aux G) G [].
 
-Definition is_head (G G':map_cfg) (b:blk) :=
-  G' ≡ (remove b.(blk_id) G) /\ wf_map_cfg G' /\
-  MapsTo b.(blk_id) b G /\ Empty (predecessors b.(blk_id) G).
+Definition head_sem (G G':map_cfg) (b:blk) :=
+  G' ≡ (remove_id b G) /\ wf_map_cfg G' /\
+  MapsTo_id b G /\ Empty (predecessors b.(blk_id) G).
+
+(* Lemmas *)
 
 Lemma Proper_predecessor_aux:
-  forall id, Proper (eq ==> Logic.eq ==> Equal ==> Equal) (predecessors_aux id).
+  forall id, Proper (eq' ==> Logic.eq ==> Logic.eq) (predecessors_aux id).
 Proof.
-  intros id idB idB' H B B' H0 x1 y1 H1 y2. apply eq_eq in H. subst B' idB'.
-  unfold predecessors_aux. remember (is_predecessor id B) as b. induction b.
-  - apply find_m. reflexivity. apply add_m; trivial. reflexivity.
-  - apply find_m; trivial. reflexivity.
-Qed.
-
-Lemma transpose_neqkey_predecessor_aux:
-    forall id, transpose_neqkey Equal (predecessors_aux id).
-Proof.
-  intros id idB idB' B B' G H id'.
-  unfold predecessors_aux. remember (is_predecessor id B) as b. remember (is_predecessor id B') as b'.
-  induction b, b'; trivial.
-  apply find_m. reflexivity. now apply swap_add.
+  now intro.
 Qed.
 
 #[global] Hint Resolve Proper_predecessor_aux : core.
-#[global] Hint Resolve transpose_neqkey_predecessor_aux : core.
 
 Lemma predecessors_in: forall G id id', In id (predecessors id' G) -> In id G.
 Proof.
-  unfold predecessors. intros G id id'. eapply fold_rec_bis.
-  - intros G1 G2 G3 He Him Hi. eapply In_m. reflexivity. symmetry.
-    apply He. apply Him. apply Hi.
-  - trivial.
-  - intros idb B G1 G2 Hm Hni Him Hip.
-    unfold predecessors_aux in Hip. remember (is_predecessor id' B) as b. induction b.
-    apply add_in_iff in Hip as [Hip|Hip].
-    * apply add_in_iff. now left.
-    * apply add_in_iff. right. now apply Him.
-    * apply add_in_iff. right. now apply Him.
+  intros G id id' Hp. apply in_mapsto_iff in Hp as [B Hp]. apply in_mapsto_iff. exists B.
+  apply filter_iff in Hp as [H _]; auto.
 Qed.
 
-Lemma predecessors_aux_empty_acc: forall G id id' acc,
-  In id (predecessors id' G) ->
-  In id (fold (predecessors_aux id') G acc).
+Lemma add_predecessor: forall (A B: blk) G G', wf_map_cfg G -> MapsTo_id A G ->
+  (predecessors B.(blk_id) (remove_id A G)) ≡ G' -> successors A = [B.(blk_id)] ->
+  (predecessors B.(blk_id) G) ≡ (add_id A G').
 Proof.
-  unfold predecessors. intros G id id'. eapply fold_rec_bis.
-  intros G1 G2 G3 He H1 acc H3.
-  - eapply In_m. reflexivity. 2:apply H1.
-    apply fold_Equal; auto. now symmetry. trivial.
-  - intros acc H. now apply empty_in_iff in H.
-  - intros idB B G1 G2 Hm Hni Him acc Hip.
-    unfold predecessors_aux in Hip.
-    eapply In_m. reflexivity.
-    assert (H:  (fold (predecessors_aux id') (add idB B G2) acc) ≡
-                ((predecessors_aux id') idB B (fold (predecessors_aux id') G2 acc))
-           ).
-    apply fold_add; auto. apply H.
-    unfold predecessors_aux at 1. remember (is_predecessor id' B) as b. induction b.
-    * apply add_in_iff in Hip as [Hip|Hip]. apply add_in_iff. now left.
-      apply add_in_iff. right. now apply Him.
-    * now apply Him.
-Qed. 
-
-Lemma add_predecessor: forall (A B: blk) G, wf_map_cfg G -> MapsTo (blk_id A) A G ->
-  Empty (predecessors B.(blk_id) (remove A.(blk_id) G)) -> successors A = [B.(blk_id)] ->
-  (predecessors B.(blk_id) G) ≡ (add A.(blk_id) A empty).
-Proof.
-  intros. remember (remove (elt:=blk) (blk_id A) G) as G'.
-  assert (H': G ≡ (add A.(blk_id) A G')).
-  {
-    apply add_remove_elim2. trivial. rewrite HeqG'. reflexivity.
-  }
-  unfold predecessors. erewrite fold_Equal;auto. 2: apply H'.
-  etransitivity.
-    - assert (H3: (fold (predecessors_aux (blk_id B)) (add (blk_id A) A G') empty) ≡
-              (predecessors_aux (blk_id B) (blk_id A) A (fold (predecessors_aux (blk_id B)) G' empty))
-             ).
-    {
-      apply fold_add; auto.
-      rewrite HeqG'. apply remove_1. reflexivity.
-    }
-    apply H3.
-  - etransitivity.
-    * apply Proper_predecessor_aux. reflexivity. reflexivity. apply Eempty. apply H1.
-    * unfold predecessors_aux. unfold is_predecessor. rewrite H2. cbn.
-      induction (raw_id_eq_dec (blk_id B) (blk_id B)). reflexivity. contradiction.
+  intros A B G G' Hwf HA He Hs. rewrite Equal_mapsto_iff in He. setoid_rewrite filter_iff in He; auto.
+  apply Equal_mapsto_iff. intros idC C. setoid_rewrite filter_iff; auto. split.
+  - intros [HmC Hp]. case (eq_dec A.(blk_id) idC); unfold eq; intro Heq.
+    * apply eq_eq in Heq. assert (A=C). eapply MapsTo_fun. apply HA. now rewrite Heq.
+      subst. now apply add_1.
+    * apply add_2; trivial. apply He. split;trivial. now apply remove_2.
+  - intro HC. case (eq_dec A.(blk_id) idC); unfold eq; intro Heq.
+    * apply eq_eq in Heq. assert (A=C). eapply MapsTo_fun. 2: apply HC. apply add_1. now subst.
+      subst. split; trivial. unfold predecessors_aux. unfold is_predecessor. rewrite Hs.
+      cbn. case (raw_id_eq_dec (blk_id B) (blk_id B)); auto.
+    * split.
+      + eapply remove_3. apply He. eapply add_3. 2: apply HC. trivial.
+      + apply He. eapply add_3. 2: apply HC. trivial.
 Qed.
 
-Lemma is_head_eq:
-  forall G G' H H' A,
-  G ≡ H -> G' ≡ H' ->
-  is_head G G' A -> is_head H H' A.
+Lemma remove_predecessor:
+  forall id A G, wf_map_cfg G -> MapsTo_id A G -> (predecessors id G) ≡ (single A) ->
+  (predecessors id (remove_id A G)) ≡ empty.
 Proof.
-  unfold is_head. intros G G' H H' B He He' [Her [Hwf' [Hm Hp]]]. repeat split.
-  - etransitivity. 2:etransitivity.
-    * symmetry. apply He'.
-    * apply Her.
-    * eapply remove_m. reflexivity. trivial.
-  - eapply wf_map_cfg_eq. apply He'. trivial.
-  - eapply MapsTo_m. reflexivity. reflexivity. symmetry. apply He. trivial.
-  - apply Eempty. etransitivity. unfold predecessors. apply fold_Equal; auto.
-    symmetry. apply He. now apply Eempty.
+  intros id A G Hwf HA Hp. rewrite Equal_mapsto_iff in Hp. setoid_rewrite filter_iff in Hp; auto.
+  apply Equal_mapsto_iff. intros idC C. setoid_rewrite filter_iff; auto. split.
+  - intros [HmC HpC]. case (eq_dec A.(blk_id) idC); unfold eq; intro Heq.
+    * apply eq_eq in Heq. assert (A=C). eapply MapsTo_fun. apply HA. rewrite Heq. eapply remove_3.
+      apply HmC. contradict HmC. intro. eapply remove_mapsto_iff. apply H0. now subst.
+    * eapply add_3. apply Heq. apply Hp. split; trivial. eapply remove_3. apply HmC.
+  - intro HC. contradict HC. intro HC. eapply empty_mapsto_iff. apply HC.
 Qed.
 
-Lemma heads_correct: forall G G' b, wf_map_cfg G -> ((b, G') ∈ (heads G) <-> is_head G G' b).
+Lemma heads_correct:
+  forall G G' b, wf_map_cfg G ->
+  (b, G') ∈ (heads G) <-> head_sem G G' b.
 Proof.
 Admitted.
