theories/Branch.v
@@ -1,0 +1,25 @@
+From Vellvm Require Import Syntax ScopeTheory Semantics.
+From ITree Require Import ITree Eq.
+Require Import FSets.FMapAVL FSets.FMapFacts.
+Require Import List.
+Import ListNotations.
+From Pattern Require Import IdModule MapCFG.
+Import Map MapF MapF.P MapF.P.F.
+Import IdOT MapCFG.
+
+Definition branches_aux (G: map_cfg) id b acc : list (blk*bid*bid*map_cfg) := match b.(blk_term) with
+    | TERM_Br _ l r => (b, l, r, (remove id (remove l (remove r G))))::acc
+    | _ => acc
+end.
+
+Definition branches (G: map_cfg): list (blk*bid*bid*map_cfg) := fold (branches_aux G) G [].
+
+Definition is_branch (G G': map_cfg) B l r :=
+    exists e L R, MapsTo_id B G /\ MapsTo l L G /\ MapsTo r R G /\
+    G' ≡ (remove_id B (remove l (remove r G))) /\ B.(blk_term) = TERM_Br e l r.
+
+Lemma branches_correct:
+    forall G G' b l r, wf_map_cfg G ->
+    ((b,l,r, G') ∈ (branches G) <-> is_branch G G' b l r).
+Proof.
+Admitted.
