theories/Denotation.v
@@ -1,0 +1,33 @@
+From Vellvm Require Import Syntax ScopeTheory Semantics.
+From ITree Require Import ITree Eq.
+From Pattern Require Import IdModule MapCFG Patterns BlockFusion.
+Require Import FSets.FMapAVL FSets.FMapFacts.
+Require Import List.
+Import TopLevelBigIntptr InterpretationStack.
+Import ListNotations.
+Import Map MapF MapF.P MapF.P.F.
+Import IdOT MapCFG Head Focus Block Patterns.
+
+(* Denotation definitions *)
+
+Definition ocfg_to_map_cfg (g: ocfg) := List.fold_right (fun b => add_id b) empty g.
+
+Definition map_cfg_to_ocfg (g : map_cfg): ocfg := List.map snd (elements g).
+
+Definition denotation_map_cfg (g : map_cfg) fto :ITreeDefinition.itree instr_E (bid * bid + uvalue) := (denote_ocfg (map_cfg_to_ocfg g)) fto.
+
+(* Block Fusion *)
+
+Definition fusion_code (A B: blk): code dtyp. Admitted.
+
+Definition fusion_comments (A B: blk): option (list String.string). Admitted.
+
+Definition fusion (A B: blk): blk :=
+  mk_block A.(blk_id) A.(blk_phis) (fusion_code A B) B.(blk_term) (fusion_comments A B).
+
+Theorem FusionCorrect (G G' G'':map_cfg) A B f to:
+  wf_map_cfg G -> to <> B.(blk_id) -> f <> A.(blk_id) ->
+  (A, (B, G')) ∈ (MatchAll (BlockFusion □) G) ->
+  denotation_map_cfg G (f, to) ≈
+  denotation_map_cfg (update G' (single (fusion A B))) (f, to).
+Admitted.
